semantics/chorTypeScript.sml
@@ -5,24 +5,25 @@ open chorLangTheory
 val _ = new_theory "chorType";
 
 
-Datatype:
-  type = typeL | unitT
+Inductive chorTypecheckOK:
+[~nil:] ∀ Γ Θ. chorTypecheckOK Γ Θ Nil
+[~com:] ∀ Γ Θ p1 v1 p2 v2 c ty. FLOOKUP Γ (v1,p1) = SOME strT ∧
+                                FLOOKUP Γ (v2,p2) = SOME strT ∧
+                                ({p1;p2} ⊆ Θ) ∧
+                                chorTypecheckOK Γ Θ c ⇒
+                                chorTypecheckOK Γ Θ (Com p1 v1 p2 v2 c)
+[~sel:] ∀ Γ Θ p1 p2 b c ty. ({p1;p2} ⊆ Θ) ∧ chorTypecheckOK Γ Θ c ⇒
+                            chorTypecheckOK Γ Θ (Sel p1 b p2 c)
+[~if:] ∀ Γ Θ v p c1 c2 ty. FLOOKUP Γ (v,p) = SOME boolT ∧
+                           chorTypecheckOK Γ Θ c1 ∧ chorTypecheckOK Γ Θ c2 ⇒
+                           chorTypecheckOK Γ Θ (IfThen v p c1 c2)
+[~let:] ∀ Γ Θ v p e c ety. typecheck (localise Γ p) e ety ∧
+                           chorTypecheckOK (Γ |+ ((v,p), ety)) Θ c ⇒
+                           chorTypecheckOK Γ Θ (Let v p e c)
+[~fix:] ∀ Γ Θ c. chorTypecheckOK Γ (Θ ∪ {dn}) c ⇒ chorTypecheckOK Γ Θ (Fix dn c)
 End
 
-Inductive chorTypecheck:
-[~nil:] ∀ Γ Θ. chorTypecheck Γ Θ Nil unitT
-[~com:] ∀ Γ Θ p1 v1 p2 v2 c ty. FLOOKUP Γ (v1,p1) = SOME strT ∧ ({p1,p2} ⊆ Θ) ∧
-                                chorTypecheck Γ Θ c ty ⇒
-                                chorTypecheck Γ Θ (Com p1 v1 p2 v2 c) ty
-[~sel:] ∀ Γ Θ p1 p2 b c ty. ({p1,p2} ⊆ Θ) ∧ chorTypecheck Γ Θ c ty ⇒
-                            chorTypecheck Γ Θ (Sel p1 b p2 c) ty
-[~if:] ∀ Γ Θ v p c1 c2 ty. FLOOKUP Γ (v,p) = SOME boolT ∧
-                           chorTypecheck Γ Θ c1 ty ∧ chorTypecheck Γ Θ c2 ty ⇒
-                           chorTypecheck Γ Θ (IfThen v p c1 c2) ty
-[~let:] ∀ Γ Θ v p e c ety ty. typecheck (localise Γ p) e ety ∧
-                              chorTypecheck (Γ |+ ((v,p), ety)) Θ c ty ⇒
-                              chorTypecheck Γ Θ (Let v p e c) ty
-End
+(* chorEnvtype *)
 
 val _ = export_theory();
 
